src/ssrseq.v
@@ -63,3 +63,5 @@ Proof.
   rewrite -[in X in _ = X]Hin'. rewrite index_uniq => //.
   move: Hin. by rewrite size_zip leq_min => /andP[H1 H2].
 Qed.
+
+
